YulEvmCompiler/Optimizer/Implementation/StackLayout.lean
@@ -19,8 +19,8 @@ namespace YulEvmCompiler.Optimizer
 open YulSemantics
 open YulSemantics.EVM
 
-variable {calls : ExternalCalls} {creates : ExternalCreates}
-local notation "D" => evmWithExternal calls creates ExternalGas.any
+variable {calls : ExternalCalls} {creates : ExternalCreates} {gasOracle : ExternalGas}
+local notation "D" => evmWithExternal calls creates gasOracle
 
 /-! ### Expression-pressure scheduling
 
